web/src/host/vir-js-value-bindings.js
@@ -11,6 +11,7 @@ export function createJsValueHostBindings() {
     bindings[`${target}.value`] = (value) => codec.fromJs(value);
   }
   bindings["js.string.owned"] = jsStringValue;
+  bindings["js.string.length"] = (value) => value.length;
   bindings["js.string.fromAny"] = (value) => {
     if (typeof value !== "string") {
       throw new TypeError("js.string.fromAny expects a primitive JavaScript string");
